$$y'''-6y''+9y'=xe^{3x}+e^{3x}\cos{2x}$$
$$y''+3y'+2y=\frac{1}{e^x+1}$$
$$ y''+2y'+y=3e^{-x}\sqrt{x+1}$$
$$ y'=f(x)g(y)$$
$$x^2y^2y'+1=y$$
$$x^2y^2\frac{dy}{dx}=y-1$$
$$x^2y^2dy=(y-1)~dx$$
$$\int\frac{y^2}{y-1}~dy=\int\frac{dx}{x^2}$$


$$  \begin{cases}
    \dot{x}=y+2~e^t,\\
    \dot{y}=x+t^2.
\end{cases}$$ 
$$  \begin{cases}
    \dot{x}=x+2y,\\
    \dot{y}=x-5~\sin{t}.
\end{cases}$$ 
$$ \dot{x}=Ax,~
A=\begin{pmatrix} 
    3 & 0  \\ 
    0 & 3 
    \end{pmatrix}.$$
 $$ \dot{x}=Ax,~
A=\begin{pmatrix}
        2 & -1 & -1  \\ 
        1 & 0 & -1 \\ 
        3 & -1 & -2 
        \end{pmatrix}.$$